wip

libcrux-ml-dsa/proofs/fstar/extraction/Libcrux_ml_dsa.Simd.Avx2.Arithmetic.fst
@@ -88,7 +88,7 @@ let montgomery_multiply_by_constant
   in
   Libcrux_intrinsics.Avx2.mm256_blend_epi32 (mk_i32 170) res02_shifted res13
 
-let montgomery_multiply_spec__i32_extended64_mul (x y: i32) : i64 =
+unfold let montgomery_multiply_spec__i32_extended64_mul (x y: i32) : i64 =
   (cast (x <: i32) <: i64) *! (cast (y <: i32) <: i64)
 
 let montgomery_multiply_spec (x y: i32) : i32 =
@@ -117,7 +117,55 @@ let montgomery_multiply_spec (x y: i32) : i32 =
   in
   Core.Num.impl_i32__wrapping_sub lhs rhs
 
-[@@FStar.Tactics.postprocess_with ( Core_models.Core_arch.X86.Interpretations.Int_vec.Lemmas.flatten_circuit )]
+let montgomery_multiply_spec_rw (x y: i32) : Lemma ((let x_mul_y:i64 = montgomery_multiply_spec__i32_extended64_mul x y in
+  let lhs:i32 = cast (x_mul_y >>! mk_i32 32 <: i64) <: i32 in
+  let rhs:i32 =
+    cast (((cast (cast (montgomery_multiply_spec__i32_extended64_mul (cast (x_mul_y <: i64) <: i32)
+                      (cast (Libcrux_ml_dsa.Simd.Traits.v_INVERSE_OF_MODULUS_MOD_MONTGOMERY_R <: u64
+                          )
+                        <:
+                        i32)
+                    <:
+                    i64)
+                <:
+                i32)
+            <:
+            i64) *!
+          (cast (Libcrux_ml_dsa.Simd.Traits.v_FIELD_MODULUS <: i32) <: i64)
+          <:
+          i64) >>!
+        mk_i32 32
+        <:
+        i64)
+    <:
+    i32
+  in
+  Core.Num.impl_i32__wrapping_sub lhs rhs) == montgomery_multiply_spec x y)
+  = ()
+
+[@@FStar.Tactics.postprocess_with ( fun _ -> 
+  let open Tactics.Circuits in
+  let open FStar.Tactics in
+  let open Core_models.Core_arch.X86.Interpretations.Int_vec.Lemmas in
+  flatten_circuit_aux
+      [
+          "Core_models";
+          "FStar.FunctionalExtensionality";
+          `%Rust_primitives.cast_tc; `%Rust_primitives.unsize_tc;
+          "Core.Ops"; `%(.[]);
+          `%Core_models.Abstractions.Bitvec.Int_vec_interp.impl__into_i32x8;
+          `%Core_models.Abstractions.Bitvec.Int_vec_interp.impl_1__into_i64x4;
+      ]
+      (top_levels_of_attr (` v_LIFT_LEMMA ))
+      (top_levels_of_attr (` Core_models.Abstractions.Bitvec.Int_vec_interp.v_SIMPLIFICATION_LEMMA ))
+      (top_levels_of_attr (` v_ETA_MATCH_EXPAND ))
+      (mk_dbg "");
+  dump "AAAA";
+  l_to_r [`montgomery_multiply_spec_rw];
+  trefl ();
+  ()
+  // Core_models.Core_arch.X86.……¬…Interpretations.Int_vec.Lemmas.flatten_circuit
+)]
 
 let montgomery_multiply (lhs rhs: Core_models.Abstractions.Bitvec.t_BitVec (mk_u64 256))
     : Core_models.Abstractions.Bitvec.t_BitVec (mk_u64 256) =
@@ -170,7 +218,43 @@ let montgomery_multiply (lhs rhs: Core_models.Abstractions.Bitvec.t_BitVec (mk_u
   in
   lhs
 
-let hey: Lemma (e_ee_1__impl__to_i32x8 (montgomery_multiply lhs rhs) 0 == montgomery_multiply_spec (e_ee_1__impl__to_i32x8 lhs 0) (e_ee_1__impl__to_i32x8 rhs 0)) = ()
+module BV_LEMMAS = Core_models.Abstractions.Bitvec.Int_vec_interp
+
+
+///Lemma that asserts that applying BitVec :: < 256 > :: from and then i32x8 :: from is the identity.
+let e_ee_1__lemma_cancel_iv'
+  (x: Core_models.Abstractions.Funarr.t_FunArray (mk_u64 8) i32) 
+  arg
+  : Lemma
+      (ensures
+        (BV_LEMMAS.e_ee_1__impl__to_i32x8 (BV_LEMMAS.e_ee_1__impl__from_i32x8 x
+              <:
+              Core_models.Abstractions.Bitvec.t_BitVec (mk_u64 256))
+          <:
+          Core_models.Abstractions.Funarr.t_FunArray (mk_u64 8) i32) arg ==
+        x arg)
+      [
+        SMTPat
+        ((BV_LEMMAS.e_ee_1__impl__to_i32x8 (BV_LEMMAS.e_ee_1__impl__from_i32x8 x
+              <:
+              Core_models.Abstractions.Bitvec.t_BitVec (mk_u64 256))
+          <:
+          Core_models.Abstractions.Funarr.t_FunArray (mk_u64 8) i32) arg)
+      ]
+      = admit ()
+
+
+let hey lhs rhs: squash (
+        Core_models.Abstractions.Bitvec.Int_vec_interp.e_ee_1__impl__to_i32x8 (montgomery_multiply lhs rhs) (mk_u64 0)
+     == montgomery_multiply_spec 
+          (Core_models.Abstractions.Bitvec.Int_vec_interp.e_ee_1__impl__to_i32x8 lhs (mk_u64 0)) 
+          (Core_models.Abstractions.Bitvec.Int_vec_interp.e_ee_1__impl__to_i32x8 rhs (mk_u64 0))
+    ) = _ by (
+      let open FStar.Tactics in
+      norm [iota; primops; delta_only [`%montgomery_multiply]; zeta];
+      l_to_r [`e_ee_1__lemma_cancel_iv'];
+      dump "goal"
+    )
 
 let shift_left_then_reduce
       (v_SHIFT_BY: i32)
